wip, refactoring AbstractField and Field
solved a lot of slow program_goal generations

src/Bedrock/Field/Synthesis/Examples/BLS12_G1.v
@@ -7,12 +7,13 @@ Require Import Crypto.Arithmetic.Partition.
 Require Import Crypto.Arithmetic.WordByWordMontgomery.
 Require Import bedrock2.NotationsCustomEntry.
 Require Import bedrock2.WeakestPrecondition.
+Require Import Crypto.Arithmetic.PrimeFieldTheorems.
 Import Syntax BinInt String List.ListNotations.
 Local Open Scope string_scope. Local Open Scope Z_scope. Local Open Scope list_scope.
 Require Import Crypto.Bedrock.Field.FieldExtensions.QuadraticFieldExtensionsSpecs.
 Require Import Rupicola.Lib.Api.
-Require Import Crypto.Bedrock.Specs.AbstractField.
-Require Import Crypto.Bedrock.Specs.PrimeField.
+Require Import Crypto.Bedrock.Specs.Field.
+Require Import Crypto.Bedrock.Specs.Field.
 Require Import Crypto.Bedrock.Field.FieldExtensions.Theory.QuadraticExtensions.
 Require Import Crypto.Bedrock.Field.Interface.Compilation2.
 Require Import Crypto.Arithmetic.UniformWeight.
@@ -23,17 +24,22 @@ Section bls12_Fp2.
 
     Existing Instances Defaults64.default_parameters Defaults64.default_parameters_ok.
 
-    Instance prime_field_parameters : PrimeField.PrimeFieldParameters.
+    Local Notation F := (F M_pos).
+
+    Instance prime_parameters : PrimeParameters := prime_parameters.
+    Instance field_names : FieldNames := field_names.
+
+    Instance field_parameters : Field.FieldParameters F.
     Proof.
         exact bls12_prime.field_parameters.
     Defined.
 
-    Instance field_parameters : AbstractField.FieldParameters.
-    Proof.
-        exact (@PrimeField.prime_field_parameters prime_field_parameters).
-    Defined.
+    (* Instance field_parameters : Field.FieldParameters. *)
+    (* Proof. *)
+    (*     exact (@Field.prime_field_parameters prime_field_parameters). *)
+    (* Defined. *)
 
-    Instance field_representation : @AbstractField.FieldRepresentation field_parameters _ _ _ _.
+    Instance field_representation : @Field.FieldRepresentation F field_parameters _ _ _ _.
     Proof.
         exact (WordByWordMontgomery.field_representation m).
     Defined.
@@ -41,11 +47,11 @@ Section bls12_Fp2.
     Check @ladderstep_body. (*Give Proper Name!!!!!!!!*)
 
     Definition bls12_G1_add := ladderstep_body.
-    (*make AbstractField.field_representation from rep in WordByWordMontgomery.*)
+    (*make Field.field_representation from rep in WordByWordMontgomery.*)
 
     Definition mpos : positive.
     Proof.
-        destruct bls12_Fp2.prime_field_parameters. eapply M_pos.
+        destruct bls12_Fp2.prime_parameters. eapply M_pos.
     Defined.
 
     (*hard-code curve-defining parameter b*)
@@ -55,7 +61,7 @@ Section bls12_Fp2.
     Definition n := felem_size_in_words.
     Definition three_b_list := Partition.partition uw n three_b.
     Definition word := BasicC64Semantics.word.
-    Definition three_b_mont := @WordByWordMontgomery.to_montgomerymod 64 n m (@m' prime_field_parameters 64) three_b_list.
+    Definition three_b_mont := @WordByWordMontgomery.to_montgomerymod 64 n m (@m' _ 64) three_b_list.
     Definition three_b_words := List.map (@word.of_Z 64 word) three_b_mont.
 
     Instance spec_of_bls12_add : spec_of (fst bls12_add).
@@ -81,7 +87,7 @@ Section bls12_Fp2.
         exact (spec_of_ladderstep three_b_words).
     Defined.
 
-    Definition three_b_F : (@F field_parameters).
+    Definition three_b_F : F.
     Proof.
         exact (ModularArithmetic.F.of_Z M_pos three_b).
     Defined.
@@ -90,14 +96,14 @@ Section bls12_Fp2.
     Proof.
         exact (spec_of_from_list three_b_F).
     Defined.
-(* 
+
     Lemma bls12_G1_ok : program_logic_goal_for_function! bls12_G1_add. (*Why does this take 7 minutes??!?!?*)
     pose proof ladderstep_correct. cbv [spec_of_G1_add].
     cbv [bls12_G1_add].
     cbv [program_logic_goal_for]. intros.
     eapply H.
         1: simpl; auto.
-        3: auto.
+        3: cbv [spec_of_bls12_mul] in H1; apply H1.
         3: cbv [spec_of_bls12_add] in H4; apply H4.
         3: cbv [spec_of_bls12_sub] in H13; apply H13.
         2: {
@@ -107,7 +113,7 @@ Section bls12_Fp2.
             cbv [CurveAdd.spec_of_from_list]. cbv [spec_of_from_list] in H0.
             assert (three_b_F = feval three_b_words).
             {
-                simpl. cbv [Representation.eval_words eval_trans three_b_F].
+                cbv [Representation.eval_words eval_trans three_b_F].
                 Require Import Crypto.Bedrock.Field.Synthesis.Examples.bls12_from_list_F.
                 pose proof (three_b_mont_mod).
                 assert (three_b_words = bls12_Fp2.three_b_words).
@@ -117,13 +123,21 @@ Section bls12_Fp2.
                     cbv. reflexivity.
                 }
                 rewrite <- H35.
+                (* unfold feval. *)
+                cbv [feval].
+                (* rewrite H34. *)
+                unfold eval_trans.
+                simpl.
                 apply f_equal.
-                cbv [word] in H34.
-                assert (@M bls12_prime.field_parameters = m).
+                (* cbv [word] in H34. *)
+                assert (@M bls12_prime.prime_parameters = m).
                 {
                     simpl. cbv [M]. cbv [m]. cbv [M_pos]. simpl. reflexivity.
                 }
                 rewrite H36 in H34.
+                unfold bls12_Fp2.three_b.
+                unfold eval_trans.
+                simpl in H34.
                 rewrite H34.
                 cbv [three_b_list]. rewrite eval_partition; [| eapply uwprops].
                 2 : {
@@ -131,20 +145,18 @@ Section bls12_Fp2.
                     clear H34 H35 H36. lia.
                 }
                 clear H H1 H2 H4 H6 H7 H9 H10 H11 H12 H13 H14 H15 H16 H17 H18 H19 H20 H21 H22 H23 H24 H25 H26 H27 H28 H29 H30 H31 H32 H33.
-                cbv [three_b bls12_Fp2.three_b]. erewrite Zmod_small; try lia.
-                cbv [n felem_size_in_words]. simpl. cbv [WordByWordMontgomery.n]. simpl.
-                cbv [uw uweight ModOps.weight]. simpl. lia.
+                cbv [three_b bls12_Fp2.three_b]. rewrite Zmod_small. 1: reflexivity. cbv. intuition subst. easy.
             }
             rewrite H34 in H0.
             eapply H0.
         }
         clear H H1 H2 H4 H6 H7 H9 H10 H11 H12 H13 H14 H15 H16 H17 H18 H19 H20 H21 H22 H23 H24 H25 H26 H27 H28 H29 H30 H31 H32 H33.
         cbv [CompilationAbstract.maybe_bounded bounded_by loose_bounds bls12_Fp2.three_b_words].
-        eassert (my_field_representation = _).
-        {
-            cbv [my_field_representation]. eauto. 
-        }
-        rewrite H.
+        (* eassert (my_field_representation = _). *)
+        (* { *)
+        (*     cbv [my_field_representation]. eauto.  *)
+        (* } *)
+        (* rewrite H. *)
         eassert (bls12_Fp2.field_representation = _).
         {
             cbv [bls12_Fp2.field_representation]. auto.
@@ -155,26 +167,26 @@ Section bls12_Fp2.
 
         assert (three_b_mont = bls12_Fp2.three_b_mont).
         {
-            pose proof (three_b_mont_eq). rewrite H2.
+            pose proof (three_b_mont_eq). rewrite H1.
             cbv [bls12_Fp2.three_b_mont bls12_Fp2.three_b_list bls12_Fp2.three_b].
             cbv [three_b_list three_b].
             assert (n = bls12_Fp2.n).
             {
                 cbv [bls12_Fp2.n]. cbv [n]. reflexivity.
             }
-            rewrite <- H4.
+            rewrite <- H2.
             assert (bls12_Fp2.uw = uw).
             {
                 cbv [bls12_Fp2.uw]. cbv [uw]. reflexivity.
             }
-            rewrite H6. reflexivity.
+            rewrite H4. reflexivity.
         }
-        rewrite <- H2.
+        rewrite <- H1.
         rewrite unsigned_of_Z_valid.
 
         2: cbv [n felem_size_in_words]; simpl.
         all: eapply three_b_mont_valid.
-Qed. *)
+Qed.
 
 End bls12_Fp2.
     (* From bedrock2 Require Import ToCString Bytedump.
