src/Bedrock/Field/Synthesis/Examples/bls12_Fp2.v
@@ -1,3 +1,4 @@
+Require Import Crypto.Bedrock.Specs.Field.
 Require Import Crypto.Bedrock.Field.Synthesis.New.WordByWordMontgomery.
 Require Import Crypto.Bedrock.Field.Synthesis.Examples.bls12_prime.
 Require Import Crypto.Bedrock.Field.Synthesis.Examples.felem_copy_p224.
@@ -5,15 +6,28 @@ Require Import Crypto.Bedrock.Field.FieldExtensions.QuadraticFieldExtensions.
 Require Import Coq.Strings.String.
 Local Open Scope string_scope. Local Open Scope Z_scope. Local Open Scope list_scope.
 
+Require Import bedrock2.NotationsCustomEntry.
+Require Import bedrock2.WeakestPrecondition.
+Require Import Crypto.Bedrock.Field.FieldExtensions.QuadraticFieldExtensionsSpecs.
+Require Import Rupicola.Lib.Api.
+Require Import Crypto.Bedrock.Field.Interface.Compilation2.
+
+Import Syntax BinInt String List.ListNotations.
+
 Section bls12_Fp2.
 
     Existing Instances Defaults64.default_parameters Defaults64.default_parameters_ok.
 
-    Existing Instance field_parameters.
+    Existing Instance prime_parameters.
+    Let prefix := "bls12_Fp2".
 
-    Definition bls12_Fp2_add := (@Fp2_add _ _ _ _ bls12_prime.field_parameters (field_representation ) (snd bls12_add) (snd felem_copy_func)).
-    Definition bls12_Fp2_mul := (@Fp2_mul _ _ _ _ bls12_prime.field_parameters (field_representation ) (snd bls12_add) (snd felem_copy_func) (snd bls12_sub) (snd bls12_mul)).
-    Definition bls12_Fp2_sub := (@Fp2_sub _ _ _ _ bls12_prime.field_parameters (field_representation ) (snd bls12_sub) (snd felem_copy_func)).
+    Instance F_names : FieldNames := field_names.
+    Instance Fp2_names : FieldNames := field_names_prefixed prefix.
+    (* Check Fp2_representation. *)
+
+    Definition bls12_Fp2_add := (@Fp2_add _ _ _ _ bls12_prime.prime_parameters F_names (field_representation ) (snd bls12_add) (snd felem_copy_func) Fp2_names).
+    Definition bls12_Fp2_mul := (@Fp2_mul _ _ _ _ bls12_prime.prime_parameters F_names (field_representation ) (snd bls12_add) (snd felem_copy_func) (snd bls12_sub) (snd bls12_mul) Fp2_names).
+    Definition bls12_Fp2_sub := (@Fp2_sub _ _ _ _ bls12_prime.prime_parameters F_names (field_representation ) (snd bls12_sub) (snd felem_copy_func) Fp2_names).
 
     (*Print rest of functions to C*)
     (* From bedrock2 Require Import ToCString Bytedump.
@@ -22,71 +36,62 @@ Section bls12_Fp2.
 
     Eval compute in c_mod. *)
 
-
-    Require Import bedrock2.NotationsCustomEntry.
-    Require Import bedrock2.WeakestPrecondition.
-    Import Syntax BinInt String List.ListNotations.
-    Local Open Scope string_scope. Local Open Scope Z_scope. Local Open Scope list_scope.
-    Require Import Crypto.Bedrock.Field.FieldExtensions.QuadraticFieldExtensionsSpecs.
-    Require Import Rupicola.Lib.Api.
-    Require Import Crypto.Bedrock.Specs.AbstractField.
-    Require Import Crypto.Bedrock.Specs.PrimeField.
-    Require Import Crypto.Bedrock.Field.FieldExtensions.Theory.QuadraticExtensions.
-    Require Import Crypto.Bedrock.Field.Interface.Compilation2.
-
     Instance spec_of_bls12_add : spec_of (fst bls12_add).
     Proof.
-        exact (@spec_of_add _ _ _ _ _ _ bls12_prime.field_parameters (field_representation)).
+        exact (@spec_of_add _ _ _ _ _ _ bls12_prime.prime_parameters F_names (field_representation)).
     Defined.
 
     Instance spec_of_bls12_Fp2_add : spec_of (fst bls12_Fp2_add).
     Proof.
-        exact (@spec_of_Fp2_add _ _ _ _ _ _ bls12_prime.field_parameters (field_representation)).
+        exact (@spec_of_Fp2_add _ _ _ _ _ _ bls12_prime.prime_parameters (field_representation) Fp2_names).
     Defined.
 
     Instance spec_of_bls12_mul : spec_of (fst bls12_mul).
     Proof.
-        exact (@spec_of_F_mul _ _ _ _ _ _ bls12_prime.field_parameters (field_representation )).
+        exact (@spec_of_F_mul _ _ _ _ _ _ bls12_prime.prime_parameters F_names (field_representation )).
     Defined.
 
     Instance spec_of_bls12_Fp2_mul : spec_of (fst bls12_Fp2_mul).
     Proof.
-        exact (@spec_of_Fp2_mul _ _ _ _ _ _ bls12_prime.field_parameters (field_representation )).
+        exact (@spec_of_Fp2_mul _ _ _ _ _ _ bls12_prime.prime_parameters (field_representation ) Fp2_names).
     Defined.
 
     Instance spec_of_bls12_sub : spec_of (fst bls12_sub).
     Proof.
-        exact (@spec_of_F_sub _ _ _ _ _ _ bls12_prime.field_parameters (field_representation )).
+        exact (@spec_of_F_sub _ _ _ _ _ _ bls12_prime.prime_parameters F_names (field_representation )).
     Defined.
 
     Instance spec_of_bls12_Fp2_sub : spec_of (fst bls12_Fp2_sub).
     Proof.
-        exact (@spec_of_Fp2_sub _ _ _ _ _ _ bls12_prime.field_parameters (field_representation )).
+        exact (@spec_of_Fp2_sub _ _ _ _ _ _ bls12_prime.prime_parameters (field_representation ) Fp2_names).
     Defined.
 
-    Instance spec_of_bls12_felem_copy : spec_of ((@felem_copy bls12_prime.field_parameters)).
+    Instance spec_of_bls12_felem_copy : spec_of ((@felem_copy F_names)).
     Proof.
-        exact (@spec_of_felem_copy _ _ _ _ _ _ field_parameters (field_representation )).
+        exact spec_of_felem_copy. (* (@Field.spec_of_felem_copy _ _ _ _ _ _ (F M_pos) field_parameters F_names (field_representation )). *)
     Defined.
-(* 
+
     Lemma bls12_Fp2_add_ok : program_logic_goal_for_function! bls12_Fp2_add.
     Proof.
-        epose proof (Fp2_add_ok). eapply H.
+        eapply Fp2_add_ok.
         Unshelve. all: try eapply Defaults64.default_parameters_ok; auto.
     Qed.
 
     Lemma bls12_Fp2_sub_ok : program_logic_goal_for_function! bls12_Fp2_sub.
     Proof.
-        epose proof (Fp2_sub_ok). cbv [bls12_Fp2_sub]. eapply (H (snd felem_copy_func) (snd bls12_sub)).
+        eapply Fp2_sub_ok.
+        (* epose proof (Fp2_sub_ok). cbv [bls12_Fp2_sub]. eapply (H (snd felem_copy_func) (snd bls12_sub)). *)
         Unshelve. all: try eapply Defaults64.default_parameters_ok; auto.
     Qed.
 
     Lemma bls12_Fp2_mul_ok : program_logic_goal_for_function! bls12_Fp2_mul.
     Proof.
-        epose proof (Fp2_mul_ok). eapply H.
+        eapply Fp2_mul_ok.
+        (* epose proof (Fp2_mul_ok). eapply H. *)
         Unshelve. all: try eapply Defaults64.default_parameters_ok; auto.
-        Set Printing All. econstructor. admit.
-    Admitted.  *)
+        econstructor.
+        (* Do we have a proof that bls12 modulus is prime? *)
+        Admitted.
 
 End bls12_Fp2.
 (* 
