src/Bedrock/Field/Synthesis/Examples/bls12_from_list_Fp2.v
@@ -1,8 +1,8 @@
 Require Import Rupicola.Lib.Api.
 Require Import Crypto.Bedrock.Field.Synthesis.Examples.bls12_prime.
 Require Import Crypto.Bedrock.Field.Synthesis.Examples.bls12_Fp2.
-Require Import Crypto.Bedrock.Specs.PrimeField.
-Require Import Crypto.Bedrock.Specs.AbstractField.
+Require Import Crypto.Bedrock.Specs.Field.
+Require Import Crypto.Bedrock.Specs.Field.
 Require Import Crypto.Bedrock.Field.Synthesis.New.WordByWordMontgomery.
 Require Import Crypto.Bedrock.Field.Synthesis.Examples.ArrayUtil.
 Require Import Crypto.Bedrock.Field.Synthesis.Examples.ScalarsUtil.
@@ -17,22 +17,36 @@ Require Import Crypto.Arithmetic.Partition.
 Require Import Crypto.Arithmetic.WordByWordMontgomery.
 Require Import Crypto.Arithmetic.WordByWordMontgomeryUtil.
 Require Import Crypto.Bedrock.Field.FieldExtensions.QuadraticFieldExtensions.
+Require Import Crypto.Bedrock.Field.FieldExtensions.QuadraticFieldExtensionsSpecs.
 
 Section FromListFp2.
 
     Existing Instances Defaults64.default_parameters
     Defaults64.default_parameters_ok.
 
-    Instance bls12_Fp2_parameters : AbstractField.FieldParameters.
-    Proof.
-        exact (@Fp2_parameters bls12_prime.field_parameters).
-    Defined.
+    Instance prime_parameters : PrimeParameters := prime_parameters.
+    Local Notation F := (F M_pos).
+    Local Notation Fp2 := (F * F)%type.
 
-    Check @AbstractField.FieldRepresentation.
-    Instance field_representation : (@AbstractField.FieldRepresentation bls12_Fp2_parameters _ _ _ _).
-    Proof.
-        exact (@Fp2_representation _ _ _ _ bls12_prime.field_parameters (@field_representation _ _ _ _ (bls12_prime.field_parameters) (@M bls12_prime.field_parameters))).
-    Defined.
+    Instance F_names : FieldNames := field_names.
+    Instance F_parameters : FieldParameters F := field_parameters.
+    Instance F_representation : FieldRepresentation F := field_representation M.
+    Instance Fp2_parameters : FieldParameters Fp2 := Fp2_parameters.
+    Instance Fp2_representation : FieldRepresentation Fp2 := Fp2_representation.
+
+    (* Existing Instance Fp2_parameters. *)
+    (* Existing Instance Fp2_representation. *)
+
+    (* Instance bls12_Fp2_parameters : FieldParameters F. *)
+    (* Proof. *)
+    (*     exact bls12_prime.field_parameters. *)
+    (* Defined. *)
+
+    (* Check @Field.FieldRepresentation. *)
+    (* Instance field_representation : (@Field.FieldRepresentation bls12_Fp2_parameters _ _ _ _). *)
+    (* Proof. *)
+    (*     exact (@Fp2_representation _ _ _ _ bls12_prime.field_parameters (@field_representation _ _ _ _ (bls12_prime.field_parameters) (@M bls12_prime.field_parameters))). *)
+    (* Defined. *)
 
     (*curve-defining parameter b*)
     Definition br := 4.
@@ -44,16 +58,17 @@ Section FromListFp2.
     Definition three_br_list := Partition.partition uw n three_br.
     Definition three_bi_list := Partition.partition uw n three_bi.
     Definition word := BasicC64Semantics.word.
-    Definition three_br_mont := Eval vm_compute in (@WordByWordMontgomery.to_montgomerymod 64 n m (@m' bls12_prime.field_parameters 64) three_br_list).
-    Definition three_bi_mont := Eval vm_compute in (@WordByWordMontgomery.to_montgomerymod 64 n m (@m' bls12_prime.field_parameters 64) three_bi_list).
+    Definition three_br_mont := Eval vm_compute in (@WordByWordMontgomery.to_montgomerymod 64 n m (@m' _ 64) three_br_list).
+    Definition three_bi_mont := Eval vm_compute in (@WordByWordMontgomery.to_montgomerymod 64 n m (@m' _ 64) three_bi_list).
     Definition three_br_words := List.map (@word.of_Z 64 word) three_br_mont.
     Definition three_bi_words := List.map (@word.of_Z 64 word) three_bi_mont.
     Definition wo := @word.of_Z 64 word 0.
 
+    Locate prime_parameters.
     Check WordByWordMontgomery.r'.
-    Existing Instance bls12_prime.field_parameters.
+    (* Existing Instance bls12_prime.field_parameters. *)
     (*Few lemmas about curve parameters*)
-    Lemma r'_correct : (2 ^ 64 * (@WordByWordMontgomery.r' 64 bls12_prime.field_parameters) mod M = 1).
+    Lemma r'_correct : (2 ^ 64 * (@WordByWordMontgomery.r' 64 _) mod M = 1).
     Proof.
         auto.
     Qed.
@@ -116,10 +131,10 @@ Section FromListFp2.
         eapply valid_max_bounds. eapply H.
     Qed.
 
-    Lemma three_br_mont_eq : three_br_mont = (@WordByWordMontgomery.to_montgomerymod 64 n m (@m' bls12_prime.field_parameters 64) three_br_list).
+    Lemma three_br_mont_eq : three_br_mont = (@WordByWordMontgomery.to_montgomerymod 64 n m (@m' _ 64) three_br_list).
     Proof. vm_compute; auto. Qed.
 
-    Lemma three_bi_mont_eq : three_bi_mont = (@WordByWordMontgomery.to_montgomerymod 64 n m (@m' bls12_prime.field_parameters 64) three_bi_list).
+    Lemma three_bi_mont_eq : three_bi_mont = (@WordByWordMontgomery.to_montgomerymod 64 n m (@m' _ 64) three_bi_list).
     Proof. vm_compute; auto. Qed.
 
     Lemma three_br_list_valid : WordByWordMontgomery.valid 64 n m three_br_list.
@@ -162,7 +177,7 @@ Section FromListFp2.
 
     Lemma three_br_mont_mod : (WordByWordMontgomery.from_montgomerymod 64
             (WordByWordMontgomery.n M 64) M (WordByWordMontgomery.m' M 64)
-            (List.map word.unsigned three_br_words)) = three_br_list.
+            (List.map Naive.unsigned three_br_words)) = three_br_list.
     Proof.
         cbv [three_br_words]. rewrite three_br_mont_eq. eapply eval_inj_list.
         2: eapply three_br_list_valid.
@@ -183,7 +198,7 @@ Section FromListFp2.
 
     Lemma three_bi_mont_mod : (WordByWordMontgomery.from_montgomerymod 64
         (WordByWordMontgomery.n M 64) M (WordByWordMontgomery.m' M 64)
-        (List.map word.unsigned three_bi_words)) = three_bi_list.
+        (List.map Naive.unsigned three_bi_words)) = three_bi_list.
     Proof.
         cbv [three_bi_words]. rewrite three_bi_mont_eq. eapply eval_inj_list.
         2: eapply three_bi_list_valid.
@@ -202,7 +217,10 @@ Section FromListFp2.
         eapply three_bi_list_valid.
     Qed.
 
-    Definition from_list_func : Syntax.func := (from_list, (["out"], (nil : list string), bedrock_func_body:(
+    Let prefix := "bls12_Fp2".
+    Instance Fp2_names : FieldNames := field_names_prefixed prefix.
+
+    Definition from_list_func : Syntax.func := (@from_list Fp2_names, (["out"], (nil : list string), bedrock_func_body:(
       coq:(cmd.store access_size.word (expr.var "out") (expr.literal (nth 0 three_br_mont 0)));
       coq:(cmd.store access_size.word (expr.op bopname.add (expr.var "out") (expr.literal (8))) (nth 1 three_br_mont 0));
       coq:(cmd.store access_size.word (expr.op bopname.add (expr.var "out") (expr.literal (16))) (nth 2 three_br_mont 0));
@@ -223,14 +241,14 @@ Section FromListFp2.
 
     Eval compute in c_mod. *)
 
-    Definition three_b_Fp2 : F.
+    Definition three_b_Fp2 : Fp2.
     Proof.
         exact (ModularArithmetic.F.of_Z M_pos three_br,ModularArithmetic.F.of_Z M_pos three_bi).
     Defined.
 
-    Instance spec_of_from_list : spec_of (from_list).
+    Instance spec_of_from_list : spec_of (@from_list Fp2_names).
     Proof.
-        exact (@spec_of_from_list _ _ _ _ _ _ bls12_Fp2_parameters field_representation three_b_Fp2) .
+        exact (@spec_of_from_list _ _ _ _ _ _ Fp2 Fp2_parameters Fp2_names Fp2_representation three_b_Fp2) .
     Defined.
 
     Ltac collect H1 H2 := let Hnew := (fresh "Hnew") in
@@ -241,7 +259,7 @@ Section FromListFp2.
 
     Lemma felem_copy_ok : program_logic_goal_for_function! from_list_func. (*Why does this take 5 minutes???!???*)
     Proof.
-        cbv [spec_of_from_list AbstractField.spec_of_from_list]. cbv [program_logic_goal_for].
+        cbv [spec_of_from_list Field.spec_of_from_list]. cbv [program_logic_goal_for].
         intros.
         
         cbv [from_list_func]. simpl.
@@ -476,33 +494,38 @@ Section FromListFp2.
             (*Apply lemma!!!*)
             cbv [three_br]. cbv [Representation.eval_words]. cbv [eval_trans].
             eapply f_equal. unfold word in H13.
-            assert (@QuadraticFieldExtensionsSpecs.fst_felem _ _ _ _ bls12_prime.field_parameters (@WordByWordMontgomery.field_representation _ _ _ _ (bls12_prime.field_parameters) (@M bls12_prime.field_parameters)) (three_br_words ++ three_bi_words) = three_br_words).
+            assert (@QuadraticFieldExtensionsSpecs.fst_felem _ _ _ _ prime_parameters F_representation (three_br_words ++ three_bi_words) = three_br_words).
             {
                 simpl. cbv [QuadraticFieldExtensionsSpecs.fst_felem firstn]. simpl.
                 cbv [three_br_words three_br_mont]. simpl. auto.
             }
-            Set Printing All.
-            cbv [word] in H14.
-            Set Printing All.
-            cbv [word].
+            (* Unset Printing Notations. *)
+            (* Set Printing Implicit. *)
+            (* cbv [word] in H14. *)
+            (* cbv [word]. *)
             rewrite H14.
             rewrite H13.
+            (* cbv [three_br_words]. *)
+            (* Set Printing All. *)
+            (* Set Printing All. *)
+            (* cbv [word]. *)
+            (* rewrite H14. *)
             cbv [three_br_list].
             rewrite eval_partition; [| eapply uwprops; lia].
             cbv [three_br n felem_size_in_words]; simpl; cbv [WordByWordMontgomery.n]. simpl.
-            cbv [uw uweight ModOps.weight]. simpl. rewrite Zmod_small; lia.
+            cbv [uw uweight ModOps.weight]. simpl. reflexivity.
             }
             pose proof three_bi_mont_mod.
             (*Apply lemma!!!*)
             cbv [three_bi]. cbv [Representation.eval_words]. cbv [eval_trans].
             eapply f_equal. unfold word in H13.
-            assert (@QuadraticFieldExtensionsSpecs.snd_felem _ _ _ _ bls12_prime.field_parameters (@WordByWordMontgomery.field_representation _ _ _ _ (bls12_prime.field_parameters) (@M bls12_prime.field_parameters)) (three_br_words ++ three_bi_words) = three_bi_words).
+            assert (@QuadraticFieldExtensionsSpecs.snd_felem _ _ _ _ _ F_representation (three_br_words ++ three_bi_words) = three_bi_words).
             {
                 simpl. cbv [QuadraticFieldExtensionsSpecs.fst_felem firstn]. simpl.
                 cbv [three_br_words three_br_mont]. simpl. auto.
             }
-            unfold word in H14. 
-            unfold word.
+            (* unfold word in H14.  *)
+            (* unfold word. *)
             rewrite H14.
             rewrite H13.
             cbv [three_bi_list].
@@ -512,7 +535,7 @@ Section FromListFp2.
         }
 
         split.
-            - assert (@QuadraticFieldExtensionsSpecs.fst_felem _ _ _ _ bls12_prime.field_parameters (@WordByWordMontgomery.field_representation _ _ _ _ (bls12_prime.field_parameters) (@M bls12_prime.field_parameters)) (three_br_words ++ three_bi_words) = three_br_words).
+            - assert (@QuadraticFieldExtensionsSpecs.fst_felem _ _ _ _ prime_parameters F_representation (three_br_words ++ three_bi_words) = three_br_words).
             {
                 simpl. cbv [QuadraticFieldExtensionsSpecs.fst_felem firstn]. simpl.
                 cbv [three_br_words three_br_mont]. simpl. auto.
@@ -520,7 +543,7 @@ Section FromListFp2.
             unfold word in *.
             rewrite H13.
             cbv [three_br_words]. rewrite unsigned_of_Z_valid; eapply three_br_mont_valid.
-            - assert (@QuadraticFieldExtensionsSpecs.snd_felem _ _ _ _ bls12_prime.field_parameters (@WordByWordMontgomery.field_representation _ _ _ _ (bls12_prime.field_parameters) (@M bls12_prime.field_parameters)) (three_br_words ++ three_bi_words) = three_bi_words).
+            - assert (@QuadraticFieldExtensionsSpecs.snd_felem _ _ _ _ prime_parameters F_representation (three_br_words ++ three_bi_words) = three_bi_words).
             {
                 simpl. cbv [QuadraticFieldExtensionsSpecs.snd_felem firstn]. simpl. auto.
             }
